AutoKchp/Internal/TotalOrder.lean
@@ -1,0 +1,29 @@
+module
+
+
+public section
+
+variable {α: Type}
+
+class TotalOrd α extends LE α where
+  le_decidable: DecidableLE α
+  eq_decidable: DecidableEq α
+  le_refl: ∀ (a: α), le a a
+  le_trans: ∀ {a b c: α}, le a b → le b c → le a c
+  le_antisymm: ∀ {a b: α}, le a b → le b a → a = b
+  le_total: ∀ (a b: α), le a b ∨ le b a
+
+
+instance [t: TotalOrd α]: DecidableLE α := t.le_decidable
+instance [t: TotalOrd α]: DecidableEq α := t.eq_decidable
+instance [t: TotalOrd α]: LT α := ⟨fun x y => x ≤ y ∧ x ≠ y⟩
+instance [t: TotalOrd α]: DecidableLT α := fun _ _ => instDecidableAnd
+
+
+theorem TotalOrd.lt_trans [t: TotalOrd α] {a b c: α} (h1: a < b) (h2: b < c): a < c :=
+  ⟨
+    t.le_trans h1.left h2.left,
+    fun eq => h1.right (t.le_antisymm h1.left (eq ▸ h2.left))
+  ⟩
+
+end
